Logic/Modal/Normal/Geach.lean
@@ -2,59 +2,232 @@ import Logic.Vorspiel.BinaryRelations
 import Logic.Modal.Normal.Formula
 import Logic.Modal.Normal.Axioms
 import Logic.Modal.Normal.Semantics
+import Logic.Modal.Normal.Completeness
+
+/-!
+  The soundness and (Kripke) completeness of Geach Logic (general term for normal modal logics by characterized by Geach axioms).
+-/
 
 namespace LO.Modal.Normal
-
-@[simp] def AxiomGeach (p: Formula α) (i j m n : ℕ) := (◇[i](□[m]p)) ⟶ (□[j](◇[n]p))
-
-@[simp] def AxiomGeach.set (i j m n : ℕ) : AxiomSet α := { AxiomGeach p i j m n | (p) }
 
 variable {α : Type u} {β : Type u}
 variable [Inhabited β]
 
-/--
-variable (rel : α → α → Prop)
-local infix:95 "≺" => rel
--/
+abbrev GeachTaple := ℕ × ℕ × ℕ × ℕ
+
+namespace GeachTaple
+
+variable (l : GeachTaple)
+
+@[simp] def i := l.1
+@[simp] def j := l.2.1
+@[simp] def m := l.2.2.1
+@[simp] def n := l.2.2.2
+
+end GeachTaple
+
+section Axioms
+
+variable {F : Type u} [ModalLogicSymbol F] [Multibox F] [Multidia F]
 
 @[simp]
-def Access (rel : Frame α) : ℕ → α → α → Prop
-| 0 => (· = ·)
-| n + 1 => λ x y => ∃ z, (rel x z ∧ Access rel n z y)
+def AxiomGeach (l : GeachTaple) (p : F) := (◇[l.i](□[l.m]p)) ⟶ (□[l.j](◇[l.n]p))
+
+def AxiomGeach.set (l : GeachTaple) : AxiomSet α := { AxiomGeach l p | (p) }
+
+class IsGeachAxiom (ax : F → F) where
+  taple : GeachTaple
+  char : ∀ p, ax p = AxiomGeach taple p
 
 @[simp]
-def GeachConfluency (i j m n : ℕ) (F : Frame α) := ∀ {x y z}, (Access F i x y) ∧ (Access F j x z) → ∃ u, (Access F m y u) ∧ (Access F n z u)
-
-namespace Formula
-
-@[simp] lemma multibox_zero : (□[0]p) = p := by simp [multibox];
-@[simp] lemma multibox_succ {n : ℕ} : (□[(n + 1)]p) = (□(□[n]p)) := by simp [multibox];
-
-@[simp] lemma multidia_zero : (◇[0]p) = p := by simp [multidia];
-@[simp] lemma multidia_succ {n : ℕ} : (◇[(n + 1)]p) = (◇(◇[n]p)) := by simp [multidia];
-
-namespace Satisfies
-
-variable {M : Model α β} {p : Formula β}
+instance : IsGeachAxiom (AxiomT : (Formula α) → (Formula α)) where
+  taple := (0, 0, 1, 0);
+  char := by simp [AxiomT];
 
 @[simp]
-lemma multibox_def : (w ⊩ᴹ[M] □[n]p) ↔ (∀ v, (Access M.frame n) w v → (v ⊩ᴹ[M] p)) := by
-  induction n generalizing w with
-  | zero => simp;
-  | succ n ih => aesop;
+instance : IsGeachAxiom (AxiomB : (Formula α) → (Formula α)) where
+  taple := (0, 1, 0, 1);
+  char := by simp [AxiomB]
 
 @[simp]
-lemma multidia_def : (w ⊩ᴹ[M] ◇[n]p) ↔ (∃ v, Access M.frame n w v ∧ (v ⊩ᴹ[M] p)) := by
-  induction n generalizing w with
-  | zero => simp;
-  | succ n ih => aesop;
+instance : IsGeachAxiom (AxiomD : (Formula α) → (Formula α)) where
+  taple := (0, 0, 1, 1);
+  char := by simp [AxiomD]
 
-end Satisfies
+@[simp]
+instance : IsGeachAxiom (Axiom4 : (Formula α) → (Formula α)) where
+  taple := (0, 2, 1, 0);
+  char := by simp [Axiom4]
 
-end Formula
+@[simp]
+instance : IsGeachAxiom (Axiom5 : (Formula α) → (Formula α)) where
+  taple := (1, 1, 0, 1);
+  char := by simp [Axiom5];
 
-theorem Geach.defines (F : Frame α) : (GeachConfluency i j m n F) ↔ (⊧ᴹ[F] (AxiomGeach.set i j m n : AxiomSet β)) := by
-  simp;
+@[simp]
+instance : IsGeachAxiom (AxiomDot2 : (Formula α) → (Formula α)) where
+  taple := (1, 1, 1, 1)
+  char := by simp [AxiomDot2]
+
+@[simp]
+instance : IsGeachAxiom (AxiomC4 : (Formula α) → (Formula α)) where
+  taple := (0, 1, 2, 0);
+  char := by simp [AxiomC4]
+
+@[simp]
+instance : IsGeachAxiom (AxiomTc : (Formula α) → (Formula α)) where
+  taple := (0, 1, 0, 0)
+  char := by simp [AxiomTc]
+
+@[simp]
+instance : IsGeachAxiom (AxiomCD : (Formula α) → (Formula α)) where
+  taple := (1, 1, 0, 0);
+  char := by simp [AxiomCD]
+
+@[simp]
+lemma eq_IsGeachAxiom [hG : IsGeachAxiom ax] : ({ ax p | p } : AxiomSet α) = (AxiomGeach.set hG.taple) := by
+  simp [hG.char];
+  aesop;
+
+@[simp]
+def GeachLogic : List (GeachTaple) → AxiomSet β
+  | [] => 𝐊
+  | x :: xs => (GeachLogic xs) ∪ (AxiomGeach.set x)
+
+@[simp]
+lemma GeachLogic.subsetK {l : List (GeachTaple)} : (𝐊 : AxiomSet β) ⊆ (GeachLogic l) := by
+  induction l with
+  | nil => simp;
+  | cons => simp; apply Set.subset_union_of_subset_left (by assumption);
+
+lemma GeachLogic.subsetK' (h : (GeachLogic l) ⊆ Λ): (𝐊 : AxiomSet β) ⊆ Λ := Set.Subset.trans GeachLogic.subsetK h
+
+class IsGeachLogic (Λ : AxiomSet β) where
+  taples : List (GeachTaple)
+  char : Λ = GeachLogic taples
+
+@[simp]
+instance : IsGeachLogic (𝐊 : AxiomSet β) where
+  taples := [];
+  char := rfl
+
+@[simp]
+instance : IsGeachLogic (𝐊𝐃 : AxiomSet β) where
+  taples := [(0, 0, 1, 1)];
+  char := by simp [LogicKD]; aesop;
+
+@[simp]
+instance : IsGeachLogic (𝐊𝐓 : AxiomSet β) where
+  taples := [(0, 0, 1, 0)];
+  char := by simp [LogicKD]; aesop;
+
+@[simp]
+instance : IsGeachLogic (𝐊𝟒 : AxiomSet β) where
+  taples := [(0, 2, 1, 0)];
+  char := by aesop;
+
+@[simp]
+instance : IsGeachLogic (𝐒𝟒 : AxiomSet β) where
+  taples := [(0, 0, 1, 0), (0, 2, 1, 0)];
+  char := by simp [LogicKT4]; aesop;
+
+@[simp]
+instance : IsGeachLogic (𝐒𝟒.𝟐 : AxiomSet β) where
+  taples := [(0, 0, 1, 0), (0, 2, 1, 0), (1, 1, 1, 1)];
+  char := by simp [LogicS4Dot2]; sorry; -- aesop;
+
+@[simp]
+instance : IsGeachLogic (𝐒𝟓 : AxiomSet β) where
+  taples := [(0, 0, 1, 0), (1, 1, 0, 1)];
+  char := by simp [LogicKT5]; aesop;
+
+@[simp]
+instance : IsGeachLogic (𝐊𝐓𝟒𝐁 : AxiomSet β) where
+  taples := [(0, 0, 1, 0), (0, 2, 1, 0), (0, 1, 0, 1)];
+  char := by simp [LogicKT4B]; aesop;
+
+end Axioms
+
+@[simp]
+def GeachConfluencyAux (l : GeachTaple) (F : Frame α) := ∀ {x y z}, (F[l.i] x y) ∧ (F[l.j] x z) → ∃ u, (F[l.m] y u) ∧ (F[l.n] z u)
+
+@[simp]
+def GeachConfluency (l : List (GeachTaple)) (rel : α → α → Prop) : Prop :=
+  match l with
+  | [] => True
+  | x :: xs => (GeachConfluencyAux x rel) ∧ (GeachConfluency xs rel)
+
+class IsGeachConfluency (P : (α → α → Prop) → Prop) where
+  taples : List (GeachTaple)
+  char : ∀ (rel : α → α → Prop), P rel ↔ GeachConfluency taples rel
+
+section GeachConfluency
+
+@[simp]
+instance : IsGeachConfluency (@Serial α) where
+  taples := [(0, 0, 1, 1)];
+  char := by simp [Symmetric]; aesop
+
+@[simp]
+instance : IsGeachConfluency (@Reflexive α) where
+  taples := [(0, 0, 1, 0)];
+  char := by simp [Reflexive];
+
+@[simp]
+instance : IsGeachConfluency (@Symmetric α) where
+  taples := [(0, 1, 0, 1)];
+  char := by simp [Symmetric]; aesop;
+
+@[simp]
+instance : IsGeachConfluency (@Transitive α) where
+  taples := [(0, 2, 1, 0)];
+  char := by simp [Transitive]; aesop
+
+@[simp]
+instance : IsGeachConfluency (@Euclidean α) where
+  taples := [(1, 1, 0, 1)];
+  char := by simp [Euclidean]; aesop
+
+@[simp]
+instance : IsGeachConfluency (@Confluent α) where
+  taples := [(1, 1, 1, 1)]
+  char := by simp [Confluent];
+
+@[simp]
+instance : IsGeachConfluency (@Extensive α) where
+  taples := [(0, 1, 0, 0)];
+  char := by
+    intros;
+    simp [Extensive];
+    constructor;
+    . intro h x y z hxy hxz;
+      have := h hxz;
+      subst hxy this;
+      trivial;
+    . intro h x y hyz;
+      have := h rfl hyz;
+      subst this;
+      trivial;
+
+@[simp]
+instance : IsGeachConfluency (@Functional α) where
+  taples := [(1, 1, 0, 0)];
+  char := by simp [Functional]; aesop
+
+@[simp]
+instance : IsGeachConfluency (@Dense α) where
+  taples := [(0, 1, 2, 0)];
+  char := by simp [Dense]; aesop
+
+lemma subset_GeachConfluency (h : l₁ ⊆ l₂) : (GeachConfluency l₂ F) → (GeachConfluency l₁ F) := by
+  induction l₁ with
+  | nil => simp;
+  | cons x xs ih => sorry;
+
+end GeachConfluency
+
+theorem AxiomGeach.defines (F : Frame α) : (GeachConfluencyAux l F) ↔ (⊧ᴹ[F] (AxiomGeach.set l : AxiomSet β)) := by
+  simp [AxiomGeach.set];
   constructor;
   . intro h p V x;
     simp only [Formula.Satisfies.imp_def'];
@@ -71,203 +244,133 @@ theorem Geach.defines (F : Frame α) : (GeachConfluency i j m n F) ↔ (⊧ᴹ[F
   . intro h x y z hi hj;
     let M : Model α β := {
       frame := F,
-      val := λ v _ => Access F m y v
+      val := λ v _ => F[l.m] y v
     }
-    have him : x ⊩ᴹ[M] ◇[i]□[m](Formula.atom default) := by aesop;
+    have him : x ⊩ᴹ[M] ◇[l.i](□[l.m](Formula.atom default)) := by aesop;
     have := h (Formula.atom default) M.val x |>.modus_ponens him;
     simp only [Formula.Satisfies.multibox_def] at this;
     obtain ⟨u, hzu, hyu⟩ := by simpa using this z hj;
     existsi u;
     exact ⟨hyu, hzu⟩;
 
-lemma _root_.Serial.geach : Serial rel ↔ GeachConfluency 0 0 1 1 rel := by
-  simp [Serial];
-
-lemma AxiomD.geach : AxiomD p = AxiomGeach p 0 0 1 1 := rfl
-
-@[simp]
-lemma AxiomD.set.geach : (AxiomD.set : AxiomSet β) = AxiomGeach.set 0 0 1 1 := rfl
-
-lemma AxiomD.defines' : (Serial F) ↔ (⊧ᴹ[F] (AxiomD.set : AxiomSet β)) := by
-  rw [Serial.geach, AxiomD.set.geach];
-  apply Geach.defines;
-
-
-lemma AxiomT.geach : AxiomT p = AxiomGeach p 0 0 1 0 := rfl
-
-@[simp]
-lemma AxiomT.set.geach : (AxiomT.set : AxiomSet β) = AxiomGeach.set 0 0 1 0 := rfl
-
-lemma _root_.Reflexive.geach : Reflexive rel ↔ GeachConfluency 0 0 1 0 rel := by
-  simp [Reflexive];
-
-lemma AxiomT.defines' : (Reflexive F) ↔ (⊧ᴹ[F] (AxiomT.set : AxiomSet β)) := by
-  rw [Reflexive.geach, AxiomT.set.geach];
-  apply Geach.defines;
-
-
-lemma AxiomB.geach : AxiomB p = AxiomGeach p 0 1 0 1 := rfl
-
-@[simp]
-lemma AxiomB.set.geach : (AxiomB.set : AxiomSet β) = AxiomGeach.set 0 1 0 1 := rfl
-
-lemma _root_.Symmetric.geach : Symmetric rel ↔ GeachConfluency 0 1 0 1 rel := by
-  simp [Symmetric];
-  aesop;
-
-lemma AxiomB.defines' : (Symmetric F) ↔ (⊧ᴹ[F] (AxiomB.set : AxiomSet β)) := by
-  rw [Symmetric.geach, AxiomB.set.geach];
-  apply Geach.defines;
-
-
-lemma Axiom4.geach : Axiom4 p = AxiomGeach p 0 2 1 0 := rfl
-
-@[simp]
-lemma Axiom4.set.geach : (Axiom4.set : AxiomSet β) = AxiomGeach.set 0 2 1 0 := rfl
-
-lemma _root_.Transitive.geach : Transitive rel ↔ GeachConfluency 0 2 1 0 rel := by
-  simp [Transitive];
-  aesop;
-
-lemma Axiom4.defines' : (Transitive F) ↔ (⊧ᴹ[F] (Axiom4.set : AxiomSet β)) := by
-  rw [Transitive.geach, Axiom4.set.geach];
-  apply Geach.defines;
-
-
-lemma Axiom5.geach : Axiom5 p = AxiomGeach p 1 1 0 1 := rfl
-
-@[simp]
-lemma Axiom5.set.geach : (Axiom5.set : AxiomSet β) = AxiomGeach.set 1 1 0 1 := rfl
-
-lemma _root_.Euclidean.geach : Euclidean rel ↔ GeachConfluency 1 1 0 1 rel := by
-  simp [Euclidean];
-  aesop;
-
-lemma Axiom5.defines' : (Euclidean F) ↔ (⊧ᴹ[F] (Axiom5.set : AxiomSet β)) := by
-  rw [Euclidean.geach, Axiom5.set.geach];
-  apply Geach.defines;
-
-
-lemma AxiomDot2.geach : AxiomDot2 p = AxiomGeach p 1 1 1 1 := rfl
-
-@[simp]
-lemma AxiomDot2.set.geach : (AxiomDot2.set : AxiomSet β) = AxiomGeach.set 1 1 1 1 := rfl
-
-lemma _root_.Confluent.geach : Confluent rel ↔ GeachConfluency 1 1 1 1 rel := by simp [Confluent];
-
-lemma AxiomDot2.defines' : (Confluent F) ↔ (⊧ᴹ[F] (AxiomDot2.set : AxiomSet β)) := by
-  rw [Confluent.geach, AxiomDot2.set.geach];
-  apply Geach.defines;
-
-
-def AxiomTc [ModalLogicSymbol F] (p : F) := p ⟶ □p
-
-def AxiomTc.set : AxiomSet α := { AxiomTc p | p }
-
-notation "𝐓𝐜" => AxiomTc.set
-
-@[simp] lemma AxiomTc.set.include : (AxiomTc p) ∈ 𝐓𝐜 := by simp [set];
-
-@[simp]
-lemma AxiomTc.set.geach : (AxiomTc.set : AxiomSet β) = AxiomGeach.set 0 1 0 0 := rfl
-
-def _root_.Extensive (F : α → α → Prop) := ∀ ⦃x y⦄, F x y → x = y
-
-lemma _root_.Extensive.geach : Extensive rel ↔ GeachConfluency 0 1 0 0 rel := by
-  simp [Extensive];
-  constructor;
-  . intro h x y z hxy hxz;
-    have := h hxz;
-    subst hxy this;
-    trivial;
-  . intro h x y hyz;
-    have := h rfl hyz;
-    subst this;
-    trivial;
-
-lemma AxiomTc.defines' : (Extensive F) ↔ (⊧ᴹ[F] (AxiomTc.set : AxiomSet β)) := by
-  rw [Extensive.geach, AxiomTc.set.geach];
-  apply Geach.defines;
-
-
-lemma _root_.Functional.geach : Functional rel ↔ GeachConfluency 1 1 0 0 rel := by simp [Functional]; aesop;
-
-lemma AxiomCD.geach : AxiomCD p = AxiomGeach p 1 1 0 0 := rfl
-
-@[simp]
-lemma AxiomCD.set.geach : (AxiomCD.set : AxiomSet β) = AxiomGeach.set 1 1 0 0 := rfl
-
-lemma AxiomCD.defines' : (Functional F) ↔ (⊧ᴹ[F] (AxiomCD.set : AxiomSet β)) := by
-  rw [Functional.geach, AxiomCD.set.geach];
-  apply Geach.defines;
-
-
-lemma AxiomC4.geach : AxiomC4 p = AxiomGeach p 0 1 2 0 := rfl
-
-@[simp]
-lemma AxiomC4.set.geach : (AxiomC4.set : AxiomSet β) = AxiomGeach.set 0 1 2 0 := rfl
-
-lemma _root_.Dense.geach : Dense rel ↔ GeachConfluency 0 1 2 0 rel := by
-  simp [Dense];
-  aesop;
-
-lemma AxiomC4.defines' : (Dense F) ↔ (⊧ᴹ[F] (AxiomC4.set : AxiomSet β)) := by
-  rw [Dense.geach, AxiomC4.set.geach];
-  apply Geach.defines;
-
-
-@[simp]
-def GeachLogic : List (ℕ × ℕ × ℕ × ℕ) → Set (Formula α)
-  | [] => 𝐊
-  | (i, j, m, n) :: xs => (GeachLogic xs) ∪ (AxiomGeach.set i j m n)
-
-lemma LogicK.geach : (LogicK : AxiomSet β) = (GeachLogic []) := rfl
-
-lemma LogicKD.geach : (LogicKD : AxiomSet β) = (GeachLogic [(0, 0, 1, 1)]) := by simp [LogicKD];
-
-def LogicKT : AxiomSet α := 𝐊 ∪ 𝐓
-
-lemma LogicKT.geach : (LogicKT : AxiomSet β) = (GeachLogic [(0, 0, 1, 0)]) := by simp [LogicKT];
-
-lemma LogicKT4.geach : (LogicKT4 : AxiomSet β) = (GeachLogic [(0, 0, 1, 0), (0, 2, 1, 0)]) := by
-  simp [LogicKT4];
-  aesop;
-
-lemma LogicS4.geach : (LogicS4 : AxiomSet β) = (GeachLogic [(0, 0, 1, 0), (0, 2, 1, 0)]) := by apply LogicKT4.geach;
-
-lemma LogicS4Dot2.geach : (LogicS4Dot2 : AxiomSet β) = (GeachLogic [(0, 0, 1, 0), (0, 2, 1, 0), (1, 1, 1, 1)]) := by
-  simp [LogicKT4, LogicS4Dot2];
-  aesop;
-
-lemma LogicS5.geach : (LogicS5 : AxiomSet β) = (GeachLogic [(0, 0, 1, 0), (1, 1, 0, 1)]) := by
-  simp [LogicKT5];
-  aesop;
-
-
-@[simp]
-def GeachConfluency.list (l : List (ℕ × ℕ × ℕ × ℕ)) (rel : α → α → Prop) : Prop :=
-  match l with
-  | [] => True
-  | (i, j, m, n) :: xs => (GeachConfluency i j m n rel) ∧ (GeachConfluency.list xs rel)
-
-
-lemma AxiomGeach.FrameClassDefinability {i j m n : ℕ} : @FrameClassDefinability α β (AxiomGeach.set i j m n) (GeachConfluency i j m n) := by
+lemma AxiomGeach.FrameClassDefinability : @FrameClassDefinability α β (AxiomGeach.set t) (GeachConfluencyAux t) := by
   intro F;
-  have := @Geach.defines α β _ i j m n F;
+  have := @AxiomGeach.defines α β _ t F;
   constructor;
   . intro h p hp; exact this.mp h p hp;
   . aesop;
 
-lemma GeachLogic.FrameClassDefinability {l : List (ℕ × ℕ × ℕ × ℕ)} : @FrameClassDefinability α β (GeachLogic l) (GeachConfluency.list l) := by
+lemma GeachLogic.FrameClassDefinability {l : List (GeachTaple)} : @FrameClassDefinability α β (GeachLogic l) (GeachConfluency l) := by
   induction l with
-  | nil => simp; apply LogicK.FrameClassDefinability;
+  | nil => apply LogicK.FrameClassDefinability;
   | cons head tail ih =>
-    simp only [GeachLogic, GeachConfluency.list, Normal.FrameClassDefinability, AxiomSetFrameClass.union];
+    simp only [GeachLogic, GeachConfluency, Normal.FrameClassDefinability, AxiomSetFrameClass.union];
     intro F;
     constructor;
     . intro h;
       exact Set.mem_inter (ih.mp h.2) (AxiomGeach.FrameClassDefinability.mp h.1)
     . intro h;
       exact ⟨AxiomGeach.FrameClassDefinability.mpr h.2, ih.mpr h.1⟩;
+
+lemma AxiomSetFrameClass.geach
+  {Λ : AxiomSet β}
+  [hG : IsGeachLogic Λ]
+  : (𝔽(Λ) : FrameClass α) = (𝔽((GeachLogic hG.taples : AxiomSet β))) := by
+  exact Set.eq_of_subset_of_subset
+    (by
+      intro F hF;
+      apply GeachLogic.FrameClassDefinability |>.mp;
+      sorry;
+    )
+    (by
+      intro F hF;
+      have := GeachLogic.FrameClassDefinability |>.mpr hF;
+      sorry;
+    );
+
+lemma AxiomSetFrameClass.geach_subset (h : l₁ ⊆ l₂) : (𝔽((GeachLogic l₂ : AxiomSet β)) : FrameClass α) ⊆ 𝔽((GeachLogic l₁ : AxiomSet β)) := by
+  intro F hF;
+  have := GeachLogic.FrameClassDefinability |>.mpr hF;
+  apply GeachLogic.FrameClassDefinability |>.mp;
+  exact subset_GeachConfluency h this;
+
+lemma AxiomSetFrameClass.geach_subset' (h : l₁ ⊆ l₂) : (𝔽(𝐊 ∪ (GeachLogic l₂ : AxiomSet β)) : FrameClass α) ⊆ 𝔽(𝐊 ∪ (GeachLogic l₁ : AxiomSet β)) := by
+  repeat rw [AxiomSetFrameClass.union];
+  gcongr;
+  apply geach_subset h;
+
+namespace CanonicalModel
+
+variable [DecidableEq β]
+variable {Λ : AxiomSet β} (hK : 𝐊 ⊆ Λ)
+
+lemma defAxiomGeach (hG : (AxiomGeach.set l) ⊆ Λ) : (GeachConfluencyAux l) (CanonicalModel Λ).frame := by
+  intro Ω₁ Ω₂ Ω₃ h;
+  replace ⟨h₁₂, h₂₃⟩ := h;
+  replace h₁₂ : ∀ {p : Formula β}, p ∈ Ω₂ → ◇[GeachTaple.i l]p ∈ Ω₁ := multiframe_dia.mp h₁₂;
+  replace h₂₃ : ∀ {p : Formula β}, p ∈ Ω₃ → ◇[GeachTaple.j l]p ∈ Ω₁ := multiframe_dia.mp h₂₃;
+  let U := (□[l.m]Ω₂) ∪ (□[l.n]Ω₃);
+  have ⟨Ω, hΩ⟩ := exists_maximal_consistent_theory (show Theory.Consistent Λ U by sorry);
+  existsi Ω;
+  simp [multiframe_box];
+  constructor;
+  . intro p hp;
+    apply hΩ;
+    left;
+    sorry;
+  . intro p hp;
+    apply hΩ;
+    right;
+    sorry;
+
+lemma defLogicGeach {l : List (GeachTaple)} (hG : (GeachLogic l) ⊆ Λ) : (GeachConfluency l) (CanonicalModel Λ).frame := by
+  induction l with
+  | nil => simp;
+  | cons head tail ih =>
+    simp only [GeachLogic, GeachConfluency];
+    constructor;
+    . apply CanonicalModel.defAxiomGeach; aesop;
+    . exact ih (by aesop);
+
+end CanonicalModel
+
+variable [DecidableEq β]
+
+def GeachLogic.CanonicalModel (l : List (GeachTaple)) := Normal.CanonicalModel (GeachLogic l : AxiomSet β)
+
+lemma GeachLogic.membership_frameclass : (CanonicalModel l).frame ∈ (𝔽((GeachLogic l : AxiomSet β)) : FrameClass (MaximalConsistentTheory (GeachLogic l : AxiomSet β))) := by
+  apply FrameClassDefinability.mp;
+  cases l with
+  | nil => simp;
+  | cons head tail =>
+    simp only [GeachConfluency, GeachLogic.CanonicalModel];
+    constructor;
+    . exact CanonicalModel.defAxiomGeach (by simp);
+    . exact CanonicalModel.defLogicGeach (by simp);
+
+theorem GeachLogic.kripkeCompletesAux (l : List (GeachTaple)) : Completeness (GeachLogic l : AxiomSet β) (𝔽((GeachLogic l : AxiomSet β)) : FrameClass (MaximalConsistentTheory (GeachLogic l : AxiomSet β))) := by
+  apply completeness_def.mpr;
+  intro Γ hConsisΓ;
+  let ⟨Ω, hΩ⟩ := exists_maximal_consistent_theory hConsisΓ;
+  existsi (CanonicalModel l).frame;
+  constructor;
+  . apply membership_frameclass;
+  . existsi (CanonicalModel l).val, Ω;
+    apply truthlemma' (by simp) |>.mpr;
+    assumption;
+
+lemma GeachLogic.kripkeCompletes {Λ : AxiomSet β} [hG : IsGeachLogic Λ] : Completeness Λ (𝔽(Λ) : FrameClass (MaximalConsistentTheory Λ)) := by
+  rw [hG.char];
+  apply GeachLogic.kripkeCompletesAux hG.taples;
+
+theorem LogicK.kripkeCompletes : Completeness (LogicK : AxiomSet β) (𝔽((LogicK : AxiomSet β)) : FrameClass (MaximalConsistentTheory (LogicK : AxiomSet β))) := GeachLogic.kripkeCompletes
+
+theorem LogicKD.kripkeCompletes : Completeness (LogicKD : AxiomSet β) (𝔽((LogicKD : AxiomSet β)) : FrameClass (MaximalConsistentTheory (LogicKD : AxiomSet β))) := GeachLogic.kripkeCompletes
+
+theorem LogicS5.kripkeCompletes : Completeness (LogicS5 : AxiomSet β) (𝔽((LogicS5 : AxiomSet β)) : FrameClass (MaximalConsistentTheory (LogicS5 : AxiomSet β))) := GeachLogic.kripkeCompletes
+
+theorem LogicS4.kripkeCompletes : Completeness (LogicS4 : AxiomSet β) (𝔽((LogicS4 : AxiomSet β)) : FrameClass (MaximalConsistentTheory (LogicS4 : AxiomSet β))) := GeachLogic.kripkeCompletes
+
+theorem LogicS4Dot2.kripkeCompletes : Completeness (LogicS4Dot2 : AxiomSet β) (𝔽((LogicS4Dot2 : AxiomSet β)) : FrameClass (MaximalConsistentTheory (LogicS4Dot2 : AxiomSet β))) := GeachLogic.kripkeCompletes
 
 end LO.Modal.Normal
