Logic/Modal/Normal/LogicSymbol.lean
@@ -29,6 +29,24 @@ class ModalDuality' (F : Type*) [ModalLogicSymbol F] where
 
 attribute [simp] ModalDuality'.box
 
+class Multibox (α : Sort _) extends Box α where
+  multibox : ℕ → α → α
+  multibox_zero : ∀ p, multibox 0 p = p
+  multibox_succ : ∀ n p, multibox (n + 1) p = □(multibox n p)
+
+notation:74 "□[" n:90 "]" p:80 => Multibox.multibox n p
+
+attribute [simp] Multibox.multibox_zero Multibox.multibox_succ
+
+class Multidia (α : Sort _) extends Dia α where
+  multidia : ℕ → α → α
+  multidia_zero : ∀ p, multidia 0 p = p
+  multidia_succ : ∀ n p, multidia (n + 1) p = ◇(multidia n p)
+
+notation:74 "◇[" n:90 "]" p:80 => Multidia.multidia n p
+
+attribute [simp] Multidia.multidia_zero Multidia.multidia_succ
+
 end LO.Modal.Normal
 
 
@@ -51,7 +69,6 @@ lemma box_union {s t : Set α} : (s ∪ t).box = s.box ∪ t.box := by simp_all 
 lemma box_mem_intro {s : Set α} {a : α} : a ∈ s → □a ∈ s.box := by simp_all [box]; aesop;
 
 lemma box_mem_iff {s : Set α} {p : α} : p ∈ s.box ↔ (∃ q ∈ s, □q = p) := by simp_all [Set.mem_image, box]
-
 
 def dia (s : Set α) : Set α := Dia.dia '' s
 
@@ -88,6 +105,30 @@ lemma predia_dia_eq (s : Set α) : s.predia.dia = { ◇p | (p : α) (_ : ◇p �
 lemma predia_dia_subset {s : Set α} : s.predia.dia ⊆ s := by simp [Set.subset_def];
 
 lemma predia_subset {s t : Set α} (h : s ⊆ t) : s.predia ⊆ t.predia := by simp_all [Set.subset_def, predia];
+
+variable [Multibox α] [Multidia α]
+
+def multibox (n : ℕ) (s : Set α) : Set α := (Multibox.multibox n) '' s
+
+@[simp] lemma multibox_zero (s : Set α) : s.multibox 0 = s := by simp [Set.multibox]
+
+@[simp]
+lemma multibox_mem_intro {s : Set α} {a : α} {n : ℕ} : a ∈ s → □[n]a ∈ s.multibox n := by
+  simp_all [Set.multibox];
+  aesop;
+
+def multidia (n : ℕ) (s : Set α) : Set α := (Multidia.multidia n) '' s
+
+lemma multidia_zero (s : Set α) : s.multidia 0 = s := by simp [Set.multidia]
+
+@[simp]
+lemma multidia_mem_intro {s : Set α} {a : α} {n : ℕ} : a ∈ s → ◇[n]a ∈ s.multidia n := by
+  simp_all [Set.multidia];
+  aesop;
+
+def multiprebox (n : ℕ) (s : Set α) := Multibox.multibox n ⁻¹' s
+
+def multipredia (n : ℕ) (s : Set α) := Multidia.multidia n ⁻¹' s
 
 end Set
 
